theories/RASimpl.v
@@ -1,9 +1,10 @@
 From Prototype Require Import Prelude Sig Constants.
-From Prototype Require LevelOne LevelTwo LevelTwoClean.
+From Prototype Require LevelOne LevelTwo LevelTwoClean LevelTwoSimp.
 From Ltac2 Require Import RedFlags Printf.
 
 Module O := LevelOne.
 Module T := LevelTwo.
+Module Simp := LevelTwoSimp.
 Module Clean := LevelTwoClean.
 
 (*********************************************************************************)
@@ -22,25 +23,34 @@ Ltac2 @external eval_subst : constr -> constr * constr := "autosubst-experiments
 (*********************************************************************************)
 
 (** Reduction flags to unfold all simplification functions (LevelTwoSimp.v). *)
-(*Ltac2 red_flags_simp () : RedFlags.t := 
+Ltac2 red_flags_simp () : RedFlags.t := 
   red_flags:(beta iota delta 
-    [esimp ssimp esimp_functional ssimp_functional
-     qsimp rsimp qsimp_functional rsimp_functional
-     substitute scomp substitute_functional scomp_functional
-     rename srcomp rename_functional srcomp_functional
-     tnat sren tnat_functional sren_functional
-     substitute_aux scomp_aux sapply_aux sup rup 
-     sapply rscomp sapply_functional rscomp_functional
-     rapply rcomp rapply_functional rcomp_functional
-     rcomp_aux rapply_aux rcons scons]).*)
-
+    [T.eq_qnat T.eq_ren T.eq_qnat_functional T.eq_ren_functional
+     Simp.dest_rspecial
+     Simp.rcons Simp.rcons_clause_2 Simp.rcons_clause_2_1 Simp.rcons_clause_2_2
+     Simp.rcons_clause_2_3 Simp.rcons_clause_2_4 Simp.rcons_clause_2_5
+     Simp.rcons_clause_2_6 
+     Simp.rapply_aux Simp.rcomp_aux 
+     Simp.rapply Simp.rcomp Simp.rapply_functional Simp.rcomp_functional 
+     Simp.qsimp Simp.rsimp Simp.qsimp_functional Simp.rsimp_functional
+     Simp.scons Simp.ctail Simp.capply_zero
+     Simp.ccomp_aux Simp.ccomp Simp.cup
+     Simp.csubstitute_aux Simp.sccomp_aux
+     Simp.csubstitute Simp.sccomp Simp.csubstitute_functional Simp.sccomp_functional
+     Simp.sup  
+     Simp.substitute Simp.scomp Simp.substitute_functional Simp.scomp_functional
+     Simp.tvar Simp.sren Simp.tvar_functional Simp.sren_functional
+     Simp.esimp Simp.ssimp Simp.esimp_functional Simp.ssimp_functional
+     Nat.eqb
+     ]).
+     
 (** Reduction flags to unfold all cleanup functions (LevelTwoClean.v). *)
 Ltac2 red_flags_clean () : RedFlags.t :=
   red_flags:(beta iota delta 
     [Clean.eclean Clean.sclean Clean.eclean_functional Clean.sclean_functional
      Clean.qclean Clean.rclean Clean.qclean_functional Clean.rclean_functional
-     Clean.clean_rename Clean.clean_substitute Clean.clean_substitute_clause_1
-     Clean.clean_rapply Clean.clean_rapply_clause_1
+     Clean.rename Clean.substitute Clean.substitute_clause_1
+     Clean.rapply Clean.rapply_clause_1
      Clean.dest_rshift Clean.dest_rshift_clause_2 Clean.dest_rshift_clause_2_clause_1
      Clean.mk_qsucc Clean.dest_var
      Clean.dest_ren Clean.dest_ren_clause_3 Clean.dest_ren_clause_3_clause_1 
